split/assumptions.v
@@ -1,0 +1,79 @@
+Require Import Split.soundness.
+
+Print Assumptions soundness.
+(**
+Axioms:
+Rdefinitions.up : Rdefinitions.R -> BinNums.Z
+Raxioms.total_order_T : forall r1 r2 : Rdefinitions.R,
+	                    {Rdefinitions.Rlt r1 r2} + {r1 = r2} +
+                        {Rdefinitions.Rgt r1 r2}
+Axioms.prop_ext : ClassicalFacts.prop_extensionality
+FunctionalExtensionality.functional_extensionality_dep : 
+forall (A : Type) (B : A -> Type) (f g : forall x : A, B x),
+(forall x : A, f x = g x) -> f = g
+Eqdep.Eq_rect_eq.eq_rect_eq : forall (U : Type) (p : U) 
+                                (Q : U -> Type) (x : Q p) 
+                                (h : p = p), x = eq_rect p Q x p h
+Raxioms.completeness : forall E : Rdefinitions.R -> Prop,
+                       Raxioms.bound E ->
+                       (exists x : Rdefinitions.R, E x) ->
+                       {m : Rdefinitions.R | Raxioms.is_lub E m}
+defs.classic : forall P : Prop, P \/ ~ P
+Classical_Prop.classic : forall P : Prop, P \/ ~ P
+Raxioms.archimed : forall r : Rdefinitions.R,
+                   Rdefinitions.Rgt (Rdefinitions.IZR (Rdefinitions.up r)) r /\
+                   Rdefinitions.Rle
+                     (Rdefinitions.Rminus
+                        (Rdefinitions.IZR (Rdefinitions.up r)) r)
+                     (Rdefinitions.IZR (BinNums.Zpos BinNums.xH))
+Raxioms.Rplus_opp_r : forall r : Rdefinitions.R,
+                      Rdefinitions.Rplus r (Rdefinitions.Ropp r) =
+                      Rdefinitions.IZR BinNums.Z0
+Raxioms.Rplus_lt_compat_l : forall r r1 r2 : Rdefinitions.R,
+                            Rdefinitions.Rlt r1 r2 ->
+                            Rdefinitions.Rlt (Rdefinitions.Rplus r r1)
+                              (Rdefinitions.Rplus r r2)
+Raxioms.Rplus_comm : forall r1 r2 : Rdefinitions.R,
+                     Rdefinitions.Rplus r1 r2 = Rdefinitions.Rplus r2 r1
+Raxioms.Rplus_assoc : forall r1 r2 r3 : Rdefinitions.R,
+                      Rdefinitions.Rplus (Rdefinitions.Rplus r1 r2) r3 =
+                      Rdefinitions.Rplus r1 (Rdefinitions.Rplus r2 r3)
+Raxioms.Rplus_0_l : forall r : Rdefinitions.R,
+                    Rdefinitions.Rplus (Rdefinitions.IZR BinNums.Z0) r = r
+Rdefinitions.Rplus : Rdefinitions.R -> Rdefinitions.R -> Rdefinitions.R
+Rdefinitions.Ropp : Rdefinitions.R -> Rdefinitions.R
+Raxioms.Rmult_plus_distr_l : forall r1 r2 r3 : Rdefinitions.R,
+                             Rdefinitions.Rmult r1 (Rdefinitions.Rplus r2 r3) =
+                             Rdefinitions.Rplus (Rdefinitions.Rmult r1 r2)
+                               (Rdefinitions.Rmult r1 r3)
+Raxioms.Rmult_lt_compat_l : forall r r1 r2 : Rdefinitions.R,
+                            Rdefinitions.Rlt (Rdefinitions.IZR BinNums.Z0) r ->
+                            Rdefinitions.Rlt r1 r2 ->
+                            Rdefinitions.Rlt (Rdefinitions.Rmult r r1)
+                              (Rdefinitions.Rmult r r2)
+Raxioms.Rmult_comm : forall r1 r2 : Rdefinitions.R,
+                     Rdefinitions.Rmult r1 r2 = Rdefinitions.Rmult r2 r1
+Raxioms.Rmult_assoc : forall r1 r2 r3 : Rdefinitions.R,
+                      Rdefinitions.Rmult (Rdefinitions.Rmult r1 r2) r3 =
+                      Rdefinitions.Rmult r1 (Rdefinitions.Rmult r2 r3)
+Raxioms.Rmult_1_l : forall r : Rdefinitions.R,
+                    Rdefinitions.Rmult
+                      (Rdefinitions.IZR (BinNums.Zpos BinNums.xH)) r = r
+Rdefinitions.Rmult : Rdefinitions.R -> Rdefinitions.R -> Rdefinitions.R
+Raxioms.Rlt_trans : forall r1 r2 r3 : Rdefinitions.R,
+                    Rdefinitions.Rlt r1 r2 ->
+                    Rdefinitions.Rlt r2 r3 -> Rdefinitions.Rlt r1 r3
+Raxioms.Rlt_asym : forall r1 r2 : Rdefinitions.R,
+                   Rdefinitions.Rlt r1 r2 -> ~ Rdefinitions.Rlt r2 r1
+Rdefinitions.Rlt : Rdefinitions.R -> Rdefinitions.R -> Prop
+Raxioms.Rinv_l : forall r : Rdefinitions.R,
+                 r <> Rdefinitions.IZR BinNums.Z0 ->
+                 Rdefinitions.Rmult (Rdefinitions.Rinv r) r =
+                 Rdefinitions.IZR (BinNums.Zpos BinNums.xH)
+Rdefinitions.Rinv : Rdefinitions.R -> Rdefinitions.R
+Raxioms.R1_neq_R0 : Rdefinitions.IZR (BinNums.Zpos BinNums.xH) <>
+                    Rdefinitions.IZR BinNums.Z0
+Rdefinitions.R1 : Rdefinitions.R
+Rdefinitions.R0 : Rdefinitions.R
+Rdefinitions.R : Set
+*)
